Add some conveniences for working with pretty terms

src/Untyped.v
@@ -1,4 +1,6 @@
 Require Import String.
+Require Import List.
+Require Import Coq.Arith.EqNat.
 
 Module Export DeBruijn.
 
@@ -6,6 +8,14 @@ Inductive lterm : Type :=
   | Var : nat -> lterm
   | Lam : lterm -> lterm
   | App : lterm -> lterm -> lterm.
+
+(** Useless, but why not have it **)
+Fixpoint gfold (f: nat -> nat) (t: lterm) : lterm :=
+  match t with
+      | Var i => Var (f i)
+      | Lam t => Lam (gfold f t)
+      | App m n => App (gfold f m) (gfold f n)
+  end.
 
 End DeBruijn.
 
@@ -18,10 +28,63 @@ Inductive pterm : Type :=
 
 End PrettyTerm.
 
-(** Useless, but why not have it **)
-Fixpoint gfold (f: nat -> nat) (t: lterm) : lterm :=
-  match t with
-      | Var i => Var (f i)
-      | Lam t => Lam (gfold f t)
-      | App m n => App (gfold f m) (gfold f n)
+(** We introduce some notational conveniences for pretty lambda terms. **)
+
+Notation "` x" := (PrettyTerm.Var x) (at level 20).
+Notation "\ x ~> M" := (PrettyTerm.Lam x M) (at level 30).
+Infix "$" := PrettyTerm.App (at level 25, left associativity).
+
+Check \"f" ~> `"f" $ \"x" ~> `"x" $ `"y" $ `"z".
+
+(** TODO There is some problem with operator precedence with [=]. *)
+Example prettier :
+  (\"f" ~> `"f" $ \"x" ~> `"x" $ `"y") =
+  PrettyTerm.Lam "f"
+    (PrettyTerm.App
+      (PrettyTerm.Var "f")
+      (PrettyTerm.Lam "x"
+        (PrettyTerm.App
+          (PrettyTerm.Var "x")
+          (PrettyTerm.Var "y")))).
+Proof. simpl. reflexivity. Qed.
+
+(** Since we don't really want to work with pretty (named) terms, we provide a function
+    [dename] for converting pretty terms to De Bruijn terms.
+*)
+
+Fixpoint lookup (s: string) (ls: list (string * nat)) : option nat :=
+  match ls with
+  | nil => None
+  | (x, n) :: t => if string_dec x s then Some n else lookup s t
   end.
+
+Fixpoint hide (s: string) (ls: list (string * nat)) : list (string * nat) :=
+  match ls with
+  | nil => (s, 0) :: nil
+  | (x, n) :: t => if string_dec x s then (x, 0) :: t else (x, n + 1) :: hide s t
+  end.
+
+Fixpoint dename1 (t: PrettyTerm.pterm) (binds: list (string * nat)) : lterm :=
+  match t with
+  | PrettyTerm.Var s => match lookup s binds with
+             | Some n => Var n
+             | None => Var 0
+             end
+  | PrettyTerm.Lam s t => Lam (dename1 t (hide s binds))
+  | PrettyTerm.App t1 t2 => App (dename1 t1 binds) (dename1 t2 binds) 
+  end.
+
+Definition dename (t : PrettyTerm.pterm) : lterm :=
+  dename1 t nil.
+
+(** To convince ourselves of the correctness of [dename], let us briefly look at what
+    it does to the combinators K and S.
+*)
+
+Example k_comb : dename (\"x" ~> \"y" ~> `"x") = Lam (Lam (Var 1)).
+Proof. reflexivity. Qed.
+
+Example s_comb :
+  dename (\"x" ~> \"y" ~> \"z" ~> `"x" $ `"z" $ (`"y" $ `"z")) =
+  Lam (Lam (Lam (App (App (Var 2) (Var 0)) (App (Var 1) (Var 0))))).
+Proof. reflexivity. Qed.
